feat: add utilities to control unfolding of `let`
This should be considered as an expedient for the problem of WP size
explosion under substitution or nested ifs. They SHOULD have more
principled solutions, which, though, might take much more time to
develop than this.

Veil/Frontend/DSL/Action/Semantics/Definitions.lean
@@ -56,6 +56,23 @@ abbrev Transition (ρ σ : Type) := ρ -> σ -> σ -> Prop
 
 end Types
 
+/-! ## Sharing barriers -/
+
+/-- A deterministic `let` wrapper used as a sharing barrier during WP generation.
+
+Unlike Lean's ordinary `let`, this should only be unfolded by dedicated rules
+late in the verification pipeline. -/
+def letEq (a : α) (f : α → β) : β := f a
+
+theorem letEq_to_forall (a : α) (p : α → Prop) : letEq a p = (∀ b, a = b → p b) := by
+  unfold letEq ; grind
+
+/-- Equality packaged as a non-substituting predicate for Veil `veil_let`. -/
+def eqWithoutSubst (a b : α) : Prop := a = b
+
+-- CHECK Maybe remove later
+instance [inst : DecidableEq α] : Decidable (eqWithoutSubst (a : α) b) := inst a b
+
 /-! ## Theory  -/
 section Theory
 
